src/coq/Refinement.v
@@ -111,8 +111,9 @@ Definition refine_L3 : relation (itree L3 (memory_stack * (local_env * stack * (
   := eutt refine_res3.
 
 (* Refinement for after interpreting pick. *)
+(* SAZ: we still want the "bigger" set to be on the left so every thing in ts' should be found in ts, right? *)
 Definition refine_L4 : relation ((itree L4 (memory_stack * (local_env * stack * (global_env * uvalue)))) -> Prop)
-  := fun ts ts' => forall t, ts t -> exists t', ts' t' /\ eutt refine_res3 t t'.
+  := fun ts ts' => forall t', ts' t' -> exists t, ts t /\ eutt refine_res3 t t'.
 
 (*
 Definition refine_res4 : relation (memory * (local_env * stack * (global_env * dvalue)))
@@ -120,6 +121,6 @@ Definition refine_res4 : relation (memory * (local_env * stack * (global_env * d
  *)
 
 Definition refine_L5 : relation ((itree L5 (memory_stack * (local_env * stack * (global_env * uvalue)))) -> Prop)
-  := fun ts ts' => forall t, ts t -> exists t', ts' t' /\ eutt refine_res3 t t'.
+  := fun ts ts' => forall t', ts' t' -> exists t, ts t /\ eutt refine_res3 t t'.
 
 End Make.
