src/coq/Transformations/Transformation.v
@@ -15,7 +15,8 @@ Import R.
 
 Definition transformation := mcfg dtyp -> mcfg dtyp.
 About refine_mcfg.
+About refine_mcfg.
 Definition transformation_correct (T: transformation): Prop :=
-  forall m, refine_mcfg m (T m).
+  forall dt entry args intrinsics m, refine_mcfg dt entry args intrinsics m (T m).
 
 
